define the "null" extension, prove it safeN and in the process, work out some bugs in the specification of the extension safety criteria

veric/smallstep_sim_extensions.v
@@ -1,4 +1,4 @@
-Add LoadPath "..".
+Load loadpath.
 Require Import veric.sim veric.sim_step_lemmas veric.base veric.expr.
 Require Import ListSet.
 
@@ -45,6 +45,19 @@ apply Address.EqDec_int.
 apply Address.EqDec_int.
 Qed.
 
+Section linkable.
+Variables (M W ext_state: Type) (proj_ext_state : W -> ext_state).
+
+Definition linkable (signature: extsig M ext_state) (handled: extsig M W) :=
+  (forall ef, List.In ef handled -> List.In ef signature) /\
+  (*ef:{P}{Q} (handled spec) is a subtype of ef:{P'}{Q'} (assumed by client)*)
+  (forall ef x x' P Q P' Q', 
+    spec_of ef handled x = (P, Q) -> spec_of ef signature x' = (P', Q') -> 
+    (forall args w m, P' args (proj_ext_state w) m -> P args w m) /\
+    (forall ret w m, Q ret w m -> Q' ret (proj_ext_state w) m)).
+
+End linkable.
+
 Definition link
   (M ora_state1 ora_state2: Type) 
   (sigma1: extsig M ora_state1) (sigma2: extsig M ora_state2) :=
@@ -81,13 +94,14 @@ Module Extension. Record Sig
 
     (*runnable = Some i when active w = i and i is runnable (i.e., not blocked
       waiting on an external function call)*)
-    runnable : W -> option nat;
-    runnable_active : forall w i, 
-      runnable w = Some i -> active w = i;
-    runnable_none : forall w c CS,
-      runnable w = None -> proj_core w (active w) = Some c -> 
-      csem (active w) = Some CS -> 
-      exists ef, exists args, at_external CS c = Some (ef, args);
+    runnable : G -> W -> option nat;
+    runnable_active : forall ge w i, 
+      runnable ge w = Some i -> active w = i;
+    runnable_none : forall ge w c CS,
+      runnable ge w = None -> 
+      csem (active w) = Some CS -> proj_core w (active w) = Some c -> 
+      (exists rv, safely_halted CS ge c = Some rv) \/
+      (exists ef, exists args, at_external CS c = Some (ef, args));
 
     (*a thread is no longer "at external" once the extension has returned 
       to it with the result of the external function call*)
@@ -101,22 +115,28 @@ Module Extension. Record Sig
       at_external wsem w = None -> 
       handles ef signature;
 
+    (*type W embeds the external state*)
     proj_ext_state : W -> ext_state;
     lift_pred : (ext_state -> M -> Prop) -> (W -> M -> Prop);
     proj_ext_state_pre : forall ef x P Q args w m,
       spec_of ef (link signature handled) x = (P, Q) -> 
-      P args (proj_ext_state w) m <-> lift_pred (P args) w m;
+      (P args (proj_ext_state w) m <-> lift_pred (P args) w m);
     proj_ext_state_post : forall ef x P Q ret w m,
       spec_of ef (link signature handled) x = (P, Q) -> 
-      Q ret (proj_ext_state w) m <-> lift_pred (Q ret) w m;
+      (Q ret (proj_ext_state w) m <-> lift_pred (Q ret) w m);
     ext_upd_at_external : forall ge w m w' m',
       corestep wsem ge w m w' m' -> 
       proj_ext_state w = proj_ext_state w';
 
+    (*generic injection of updated external state into a W*)
     inj_ext_state : ext_state -> W -> W;
     proj_inj : forall ora w, proj_ext_state (inj_ext_state ora w) = ora;
 
-    (*a global invariant characterizing "safe" extensions*)
+    (*csem and wsem are signature linkable*)
+    csem_wsem_linkable: linkable proj_ext_state signature handled;
+
+    (*a global invariant characterizing "safe" extensions: an projectible core 
+       is safeN*)
     all_safe (ge: G) (n: nat) (w: W) (m: M) :=
       forall i CS c, csem i = Some CS -> proj_core w i = Some c -> 
         safeN CS signature ge n (proj_ext_state w) c m
@@ -124,8 +144,9 @@ Module Extension. Record Sig
 
 End Extension. 
 
-(*an extension E is safe when all states satisfy the "all_safe" invariant*)
+Implicit Arguments Extension.Make [G W C M D ext_state].
 
+(*an extension E is safe when all states satisfy the "all_safe" invariant*)
 Section SafeExtension.
 Variables
   (G W C M D ext_state: Type) 
@@ -134,10 +155,10 @@ Variables
   (signature: extsig M ext_state)
   (handled: extsig M W).
 
-Notation inv := Extension.all_safe.
+Notation all_safe := Extension.all_safe.
 
 Definition safe_extension (E: Extension.Sig wsem csem signature handled) := 
-  forall ge n w m,  E.(inv) ge n w m -> 
+  forall ge n w m,  E.(all_safe) ge n w m -> 
     safeN wsem (link signature handled) ge n (E.(Extension.proj_ext_state) w) w m.
 
 End SafeExtension.
@@ -148,10 +169,11 @@ Variables
   (signature: extsig M ext_state) 
   (handled: extsig M W).
 
+(*this is somewhat vacuous now because of the defn. of linking*)
 Lemma safety_monotonicity : forall ge n ora c m,
   safeN CS (link signature handled) ge n ora c m -> 
   safeN CS signature ge n ora c m.
-Admitted.
+Proof. intros ge n; induction n; simpl; auto. Qed.
 
 End SafetyMonotonicity.
 
@@ -193,15 +215,15 @@ Proof. intros INV i CS c H2 H3; eapply safe_downward1; eauto. Qed.
 Inductive safety_criteria: Type := SafetyCriteria: forall 
   (*coresteps preserve the invariant*)
   (core_pres: forall ge n w c m CS i w' c' m', 
-    ALL_SAFE ge n w m -> 
+    ALL_SAFE ge (S n) w m -> 
     ACTIVE w = i -> THREAD i is (CS, c) in w -> 
     corestep CS ge c m c' m' -> corestep wsem ge w m w' m' -> 
     THREAD i is (CS, c') in w' /\ ALL_SAFE ge n w' m')
 
   (*corestates satisfying the invariant can corestep*)
   (core_prog: forall ge n w m i c CS, 
-    ALL_SAFE ge n w m -> 
-    ACTIVE w = i -> RUNNABLE w = Some i -> THREAD i is (CS, c) in w -> 
+    ALL_SAFE ge (S n) w m -> 
+    ACTIVE w = i -> RUNNABLE ge w = Some i -> THREAD i is (CS, c) in w -> 
     exists c', exists w', exists m', 
       corestep CS ge c m c' m' /\ corestep wsem ge w m w' m' /\
       THREAD i is (CS, c') in w')
@@ -218,27 +240,37 @@ Inductive safety_criteria: Type := SafetyCriteria: forall
         (forall j, ACTIVE w' = j -> i <> j)) \/
       (exists ret, after_external CS ret c = Some c' /\ LIFT (Q ret) w' m')))
 
-  (*"internal" states satisfying the invariant can step; moreover, core 
-     states that stay "at_external" remain unchanged*)
+  (*"handled" states satisfying the invariant can step or are safely halted; 
+     core states that stay "at_external" remain unchanged*)
   (handled_prog: forall ge n w m,
-    ALL_SAFE ge n w m -> RUNNABLE w = None -> 
-    exists w', exists m', corestep wsem ge w m w' m' /\ 
+    ALL_SAFE ge n w m -> RUNNABLE ge w = None -> 
+    at_external wsem w = None -> 
+    (exists w', exists m', corestep wsem ge w m w' m' /\ 
       forall i c CS, THREAD i is (CS, c) in w -> 
         exists c', THREAD i is (CS, c') in w' /\ 
           (forall ef args ef' args', 
             at_external CS c = Some (ef, args) -> 
-            at_external CS c' = Some (ef', args') -> c=c'))
+            at_external CS c' = Some (ef', args') -> c=c')) \/
+    (exists rv, safely_halted wsem ge w = Some rv))
+
+  (*safely halted threads remain halted*)
+  (safely_halted_halted: forall ge w m w' m' i CS c rv,
+    THREAD i is (CS, c) in w -> safely_halted CS ge c = Some rv -> 
+    corestep wsem ge w m w' m' -> 
+    THREAD i is (CS, c) in w')
 
   (*safety of other threads is preserved when handling one step of 
      blocked thread i*)
-  (handled_rest: forall ge w m w' m' c CS ef args,
+  (handled_rest: forall ge w m w' m' c CS,
     let i := ACTIVE w in THREAD i is (CS, c) in w -> 
-    at_external CS c = Some (ef, args) -> 
+    ((exists ef, exists args, at_external CS c = Some (ef, args)) \/ 
+      exists rv, safely_halted CS ge c = Some rv) -> 
     at_external wsem w = None -> 
     corestep wsem ge w m w' m' -> 
     (forall CS0 c0 j, i <> j ->  
       (THREAD j is (CS0, c0) in w' -> THREAD j is (CS0, c0) in w) /\
-      (forall n, safeN CS0 signature ge (S n) (PROJ_EXT w) c0 m -> 
+      (forall n, THREAD j is (CS0, c0) in w -> 
+                 safeN CS0 signature ge (S n) (PROJ_EXT w) c0 m -> 
                  safeN CS0 signature ge n (PROJ_EXT w') c0 m')))
 
   (*if the extended machine is at external, then the active thread is
@@ -251,8 +283,8 @@ Inductive safety_criteria: Type := SafetyCriteria: forall
       at_external CS c = Some (ef, args))
 
   (*inject the results of an external call into the extended machine state*)
-  (at_extern_ret: forall i c w m ora m' args ret c' P Q CS ef x,
-    THREAD i is (CS, c) in w -> 
+  (at_extern_ret: forall c w m ora m' args ret c' P Q CS ef x,
+    let i := ACTIVE w in THREAD i is (CS, c) in w -> 
     spec_of ef signature x = (P, Q) -> 
     P args (PROJ_EXT w) m -> Q ret ora m' -> 
     after_external CS ret c = Some c' -> 
@@ -263,8 +295,8 @@ Inductive safety_criteria: Type := SafetyCriteria: forall
 
   (*safety of other threads is preserved when returning from an external 
      function call*)
-  (at_extern_rest: forall i c w m ora w' m' args ret c' P Q CS ef x,
-    THREAD i is (CS, c) in w -> 
+  (at_extern_rest: forall c w m ora w' m' args ret c' P Q CS ef x,
+    let i := ACTIVE w in THREAD i is (CS, c) in w -> 
     spec_of ef signature x = (P, Q) -> 
     P args (PROJ_EXT w) m -> Q ret ora m' -> 
     after_external CS ret c = Some c' -> 
@@ -272,8 +304,9 @@ Inductive safety_criteria: Type := SafetyCriteria: forall
     THREAD i is (CS, c') in w' -> 
     (forall CS0 c0 j, i <> j -> 
       (THREAD j is (CS0, c0) in w' -> THREAD j is (CS0, c0) in w) /\
-      (forall ge n, safeN CS0 signature ge (S n) (PROJ_EXT w) c0 m -> 
-        safeN CS0 signature ge n (PROJ_EXT w') c0 m'))),
+      (forall ge n, THREAD j is (CS0, c0) in w -> 
+                    safeN CS0 signature ge (S n) (PROJ_EXT w) c0 m -> 
+                    safeN CS0 signature ge n (PROJ_EXT w') c0 m'))),
   safety_criteria.
 
 Lemma safety_criteria_safe : safety_criteria -> safe_extension E.
@@ -283,7 +316,7 @@ intros w m H1; simpl; auto.
 intros w m H1.
 simpl; case_eq (at_external wsem w).
 
-(*CASE 1: at_external = Some _; i.e. _really_ at_external*) 
+(*CASE 1: at_external OUTER = Some _; i.e. _really_ at_external*) 
 intros [ef args] AT_EXT.
 destruct (at_external_halted_excl wsem ge w) as [H2|H2].
 rewrite AT_EXT in H2; congruence.
@@ -302,8 +335,9 @@ exists x.
 split; auto.
 intros ret m' z' POST.
 destruct (H8 ret m' z' POST) as [c' [H10 H11]].
-specialize (at_extern_ret (ACTIVE w) c w m z' m' args ret c' 
+specialize (at_extern_ret c w m z' m' args ret c' 
   (ext_spec_pre signature ef x) (ext_spec_post signature ef x) CS ef x).
+hnf in at_extern_ret.
 spec at_extern_ret; auto.
 spec at_extern_ret; auto.
 spec at_extern_ret; auto.
@@ -324,8 +358,9 @@ rewrite PROJJ in H15; inversion H15; rewrite H9 in *.
 auto.
 (*i<>j*)
 intros Hneq _.
-specialize (at_extern_rest (ACTIVE w) c w m (PROJ_EXT w') w' m' args ret c'
+specialize (at_extern_rest c w m (PROJ_EXT w') w' m' args ret c'
   (ext_spec_pre signature ef x) (ext_spec_post signature ef x) CS ef x).
+hnf in at_extern_rest.
 spec at_extern_rest; auto.
 spec at_extern_rest; auto.
 spec at_extern_rest; auto.
@@ -338,36 +373,39 @@ eapply H17; eauto.
 destruct H16 as [H18 H19]; auto.
 eapply H1'; eauto.
 
-(*CASE 2: at_external = None; i.e., handled function*)
+(*CASE 2: at_external OUTER = None; i.e., handled function*)
 intros H2.
-destruct (safely_halted wsem ge w); auto.
-case_eq (RUNNABLE w).
+case_eq (safely_halted wsem ge w); auto.
+case_eq (RUNNABLE ge w).
 (*active thread i*)
 intros i RUN.
-generalize (runnable_active _ RUN) as ACT; intro.
+generalize (runnable_active _ _ RUN) as ACT; intro.
 rewrite <-ACT in *.
 destruct (active_csem w) as [CS CSEM].
 destruct (active_proj_core w) as [c PROJECT].
-destruct (core_prog ge n w m i c CS (all_safe_downward H1) ACT) 
+destruct (core_prog ge n w m i c CS H1 ACT) 
  as [c' [w' [m' [CORESTEP_C [CORESTEP_W [CSEM' PROJECT']]]]]]; auto.
 rewrite <-ACT; auto.
 rewrite <-ACT; auto.
-destruct (core_pres ge n w c m CS i w' c' m' (all_safe_downward H1) ACT)
+destruct (core_pres ge n w c m CS i w' c' m' H1 ACT)
  as [_ INV']; auto.
 rewrite <-ACT in *; auto.
 exists w'; exists m'; split; [auto|].
 erewrite ext_upd_at_external; eauto.
-(*active thread none*)
+(*no runnable thread*)
 intros RUN.
 destruct (active_csem w) as [CS CSEM].
 destruct (active_proj_core w) as [c PROJECT].
-destruct (handled_prog ge n w m (all_safe_downward H1) RUN) 
- as [w' [m' [CORESTEP_W CORES_PRES]]].
+destruct (handled_prog ge n w m (all_safe_downward H1) RUN H2)
+ as [[w' [m' [CORESTEP_W CORES_PRES]]]|[rv SAFELY_HALTED]].
+2: intros CONTRA; rewrite CONTRA in SAFELY_HALTED; congruence.
 exists w'; exists m'.
 split; auto.
 erewrite ext_upd_at_external; eauto; eapply IHn.
-destruct (runnable_none w RUN PROJECT CSEM) 
- as [ef [args AT_EXT]].
+destruct (runnable_none ge w RUN CSEM PROJECT) 
+ as [SAFELY_HALTED|[ef [args AT_EXT]]].
+
+(*subcase A of no runnable thread: safely halted*)
 intros j CSj cj CSEMj PROJECTj.
 set (i := ACTIVE w) in *.
 case_eq (eq_nat_dec i j).
@@ -376,7 +414,45 @@ intros Heq _; rewrite Heq in *.
 destruct (proj_exists ge j w m w' m' CORESTEP_W PROJECTj)
  as [c0 PROJECT0].
 rewrite PROJECT in PROJECT0; inversion PROJECT0; subst.
-rewrite CSEM in CSEMj; inversion CSEMj; rewrite <-H3 in *.
+rewrite CSEM in CSEMj; inversion CSEMj; rename H4 into H3; rewrite <-H3 in *.
+specialize (H1 j CS c0 CSEM PROJECT).
+simpl in H1. 
+destruct SAFELY_HALTED as [rv SAFELY_HALTED].
+destruct (@at_external_halted_excl G C M D CS ge c0) as [H4|H4]; 
+ [|congruence].
+destruct n; simpl; auto.
+destruct (safely_halted_halted ge w m w' m' j CS c0 rv) as [H6 H7]; auto.
+rewrite H7 in PROJECTj; inversion PROJECTj; subst.
+rewrite H4, SAFELY_HALTED; auto.
+(*i<>j*)
+intros Hneq _.
+destruct (CORES_PRES i c CS) as [c' [[_ PROJ'] H5]]. 
+split; auto.
+specialize (handled_rest ge w m w' m' c CS).
+hnf in handled_rest.
+spec handled_rest; auto.
+spec handled_rest; auto.
+spec handled_rest; auto.
+spec handled_rest; auto.
+destruct (handled_rest CSj cj j Hneq) as [H6 H7].
+eapply H7; eauto.
+destruct (proj_exists ge j w m w' m' CORESTEP_W PROJECTj)
+ as [c0 PROJECT0].
+specialize (H1 j CSj c0 CSEMj PROJECT0).
+destruct H6 as [H8 H9].
+split; auto.
+rewrite H9 in PROJECT0; inversion PROJECT0; subst; auto.
+
+(*subcase B of no runnable thread: at external INNER*)
+intros j CSj cj CSEMj PROJECTj.
+set (i := ACTIVE w) in *.
+case_eq (eq_nat_dec i j).
+(*i=j*)
+intros Heq _; rewrite Heq in *.
+destruct (proj_exists ge j w m w' m' CORESTEP_W PROJECTj)
+ as [c0 PROJECT0].
+rewrite PROJECT in PROJECT0; inversion PROJECT0; subst.
+rewrite CSEM in CSEMj; inversion CSEMj; rename H4 into H3; rewrite <-H3 in *.
 specialize (H1 j CS c0 CSEM PROJECT).
 simpl in H1. 
 rewrite AT_EXT in H1.
@@ -418,7 +494,7 @@ exists c''; split; auto.
 eapply safe_downward1; eauto.
 (*post case*)
 destruct H4 as [[H4 H5] H6].
-rewrite H5 in PROJECTj; inversion PROJECTj; rewrite <-H1 in *.
+rewrite H5 in PROJECTj; inversion PROJECTj; rename H7 into H1; rewrite <-H1 in *.
 destruct POST' as [ret [AFTER_EXT POST']].
 generalize (after_at_external_excl j c0 ret H4 AFTER_EXT); intros AT_EXT'.
 clear - PRE POST POST' AT_EXT' AFTER_EXT H4 H5 H6 HeqSAFELY_HALTED.
@@ -438,12 +514,12 @@ exists c3; exists m''; split; auto.
 intros Hneq _.
 destruct (CORES_PRES i c CS) as [c' [[_ PROJ'] H5]]. 
 split; auto.
-specialize (handled_rest ge w m w' m' c CS ef args).
+specialize (handled_rest ge w m w' m' c CS).
 hnf in handled_rest.
 spec handled_rest; auto.
 spec handled_rest; auto.
+left; exists ef; exists args; auto.
 spec handled_rest; auto.
-(* eapply handles_ok with (i := i); eauto.*)
 spec handled_rest; auto.
 destruct (handled_rest CSj cj j Hneq) as [H6 H7].
 eapply H7; eauto.
