veric/null_extension.v
@@ -1,0 +1,288 @@
+Load loadpath.
+Require Import msl.base
+               veric.sim veric.sim_step_lemmas veric.base veric.expr
+               veric.smallstep_sim_extensions.
+
+Set Implicit Arguments.
+
+Section NullExtSpec.
+Variables (M ext_state: Type) (ext_spec_type: AST.external_function -> Type).
+
+Definition null_extspec := Build_external_specification 
+  M AST.external_function ext_state
+  ext_spec_type
+  (fun (ef: AST.external_function) (_:ext_spec_type ef) 
+       (args: list val) (z: ext_state) (m: M) => False)
+  (fun (ef: AST.external_function) (_:ext_spec_type ef) 
+       (ret: val) (z: ext_state) (m: M) => True).
+
+End NullExtSpec.
+
+Section NullExtsig.
+Variable (M ext_state: Type) (ext_spec_type: AST.external_function -> Type).
+
+Definition null_extsig := mk_extsig nil (null_extspec M ext_state ext_spec_type).
+
+End NullExtsig.
+
+Section NullExtension.
+Variables 
+  (G C M D ext_state: Type) 
+  (csem: CoreSemantics G C M D)
+  (signature: extsig M ext_state)
+  (init_world: ext_state)
+
+  (after_at_external_excl: forall c ret c',
+    after_external csem ret c = Some c' -> at_external csem c' = None)
+  (at_external_handled: forall c ef args,
+    at_external csem c = Some (ef, args) -> handles ef signature).
+
+Definition cores := fun _:nat => Some csem.
+
+Definition extension_state := (ext_state*C)%type.
+
+Program Definition wsem: CoreSemantics G extension_state M D := 
+  Build_CoreSemantics G extension_state M D 
+  (initial_mem csem)
+  (fun ge f args => match make_initial_core csem ge f args with
+                    | None => None
+                    | Some c => Some (init_world, c)
+                    end)
+  (at_external csem oo snd)
+  (fun ret s => match after_external csem ret (snd s) with 
+                | None => None
+                | Some c => Some (fst s, c)
+                end)
+  (fun ge s => safely_halted csem ge (snd s))
+  (fun ge s m s' m' => corestep csem ge (snd s) m (snd s') m' /\ fst s=fst s')
+  _ _ _.
+Next Obligation.
+destruct q; destruct q'; unfold compose; simpl in *.
+eapply corestep_not_at_external; eauto.
+Qed.
+Next Obligation.
+destruct q; destruct q'; simpl in *.
+eapply corestep_not_halted; eauto.
+Qed.
+Next Obligation.
+destruct q; unfold compose; simpl in *.
+eapply at_external_halted_excl.
+Qed.
+
+Local Open Scope nat_scope.
+ 
+Definition proj_core (s: extension_state) (i:nat) := 
+  if eq_nat_dec i 1 then Some (snd s) else None.
+Definition active := fun _:extension_state => 1.
+Definition runnable := fun (ge: G) (s :extension_state) => 
+  match at_external csem (snd s), safely_halted csem ge (snd s) with 
+  | None, None => Some 1
+  | _, _ => None
+  end.
+Definition proj_ext_state := @fst ext_state C.
+Definition lift_pred (P: ext_state -> M -> Prop) := 
+  fun p:extension_state => P (fst p).
+Definition inj_ext_state (z: ext_state) (s: extension_state) := 
+  (z, snd s).
+
+(*Users will typically have to prove that their extension and client signatures
+   are compatible; here, we assume it since we are parametric in signature*)
+Variable null_extsig_linkable: forall S, 
+  linkable proj_ext_state S (null_extsig M (ext_state*C) 
+    (ext_spec_type signature)).
+
+Local Hint Unfold cores proj_core active runnable proj_ext_state 
+  lift_pred inj_ext_state : null_unfold.
+
+Obligation Tactic := 
+  autounfold with null_unfold;
+  intros; try solve [eexists; eauto|congruence].
+
+Program Definition null_extension := Extension.Make 
+  wsem cores signature (null_extsig _ _ (ext_spec_type signature)) 
+  proj_core _
+  active _ _
+  runnable _ _ _ _
+  proj_ext_state lift_pred _ _ _
+  inj_ext_state _ _.
+Next Obligation.
+revert H0; case_eq (eq_nat_dec i 1).
+intros -> _; exists (snd w); auto.
+congruence.
+Qed.
+Next Obligation.
+if_tac; exists (snd w); auto.
+elimtype False; apply H; auto.
+Qed.
+Next Obligation. 
+destruct (at_external csem (snd w)); try solve[congruence]. 
+destruct (safely_halted csem ge (snd w)); try solve[congruence].
+Qed.
+Next Obligation. 
+case_eq (at_external csem (snd w)); try solve[congruence]. 
+intros [ef args] H2.
+rewrite H2 in H; right; exists ef; exists args.
+inversion H0; subst; auto.
+inversion H1; subst; auto.
+intros H2; rewrite H2 in H.
+case_eq (safely_halted csem ge (snd w)). 
+intros rv H3; left; exists rv.
+inversion H0; subst.
+inversion H1; subst.
+auto.
+intros H3.
+rewrite H3 in H.
+congruence.
+Qed.
+Next Obligation. inversion H; subst; eapply after_at_external_excl; eauto. Qed.
+Next Obligation. inversion H; subst; eapply at_external_handled; eauto. Qed.
+Next Obligation. destruct w; destruct w'; simpl in *; destruct H; auto. Qed.
+Next Obligation. apply null_extsig_linkable. Qed.
+
+Section NullExtensionSafe.
+Variable (csem_det: forall ge c m c' m' c'' m'',
+           corestep csem ge c m c' m' -> corestep csem ge c m c'' m'' -> 
+           (c', m')=(c'', m'')).
+
+Lemma null_extension_safe : safe_extension null_extension.
+Proof.
+apply safety_criteria_safe; constructor; autounfold with null_unfold in *.
+
+(*1*) intros until m'; intros H1 H2 [H3 H4] H5 H6. 
+split; auto. split; auto. inversion H6; subst; simpl.
+autounfold with null_unfold in *.
+inversion H3; rewrite H7 in *.
+inversion H4; rewrite H8 in *.
+f_equal; generalize (csem_det _ _ _ _ _ _ _ H H5); inversion 1; auto.
+inversion H6; subst.
+unfold Extension.all_safe; intros i CS0 c0; inversion 1.
+rewrite H8 in *.
+intros H9; simpl in H4; autounfold with null_unfold in *; simpl in *.
+autounfold with null_unfold in *.
+inversion H4; rewrite H10 in *.
+inversion H9; rewrite H11 in *.
+if_tac in H11; try solve[congruence].
+inversion H11; rewrite H13 in *.
+eapply safe_corestep_forward; eauto.
+unfold corestep_fun; intros; eapply csem_det; eauto.
+specialize (H1 1 CS0 (snd w)); unfold proj_ext_state in H1.
+rewrite <-H0.
+assert (Extension.proj_ext_state null_extension w = fst w).
+ simpl; autounfold with null_unfold; auto.
+rewrite <-H10, <-H12; apply H1; auto.
+
+(*2*) intros until CS; intros H1 H2 H3 [H4 H5].
+spec H1 i CS c H4 H5.
+simpl in H3.
+destruct w.
+unfold runnable in H3; simpl in H3.
+case_eq (at_external csem c0).
+intros [ef args] H6.
+rewrite H6 in H3.
+simpl in H5; unfold proj_core in H5; simpl in H5; inversion H5; subst.
+congruence.
+intros H6.
+rewrite H6 in H3.
+inversion H3; subst.
+simpl in H1.
+inversion H6; subst.
+simpl in H5; unfold proj_core in H5; simpl in H5; inversion H5; subst.
+inversion H4; rewrite H7 in *.
+rewrite H2 in H1.
+rewrite <-H7 in H1.
+destruct (safely_halted csem ge c); try solve[congruence].
+destruct H1 as [c' [m' [H8 H9]]].
+exists c'; exists (e, c'); exists m'; split; auto.
+rewrite <-H7; auto.
+split; auto.
+simpl.
+split; auto.
+
+(*3*) intros until x; intros [H1 H2] H3 H4 H5 H6 H7 H8.
+simpl in H6; unfold lift_pred in H6.
+generalize (Extension.csem_wsem_linkable null_extension); intros [H9 H10].
+simpl in H10.
+specialize (H10 ef x x).
+specialize (H10 (ext_spec_pre (null_extsig M extension_state 
+  (ext_spec_type signature)) ef x)).
+specialize (H10 (ext_spec_post (null_extsig M extension_state
+  (ext_spec_type signature)) ef x)).
+specialize (H10 P Q).
+spec H10; auto.
+spec H10; auto.
+destruct H10 as [H10 H11].
+specialize (H10 args w m H6); elimtype False; auto.
+
+(*4*) intros until m; intros H1 H2 H3.
+simpl in H2; unfold runnable in H2.
+inversion H3; subst.
+unfold compose in H0;  simpl in H0.
+rewrite H0 in H2.
+case_eq (safely_halted csem ge (snd w)); intros; try solve[congruence].
+rewrite H in H2.
+right; exists i; auto.
+rewrite H in H2; congruence.
+
+(*5*) intros until rv; intros [H1 H2] H3 H4.
+split; auto.
+simpl.
+inversion H4; subst.
+apply corestep_not_halted in H.
+simpl in H2; inversion H2; subst.
+inversion H1; rewrite H7 in *.
+unfold proj_core in H6.
+if_tac in H6; try solve[congruence].
+
+(*6*) intros until CS; inversion 1; subst.
+intros H4 H5; intros until j; intros H6; split.
+intros [H7 H8]. 
+split; auto.
+simpl in H8; unfold proj_core in H8; simpl in H8; inversion H8; subst.
+simpl; unfold proj_core; simpl.
+simpl in H6; unfold active in H6.
+if_tac; auto; exfalso; apply H6; auto.
+intros n [H7 H8].
+simpl in H8; unfold proj_core in H8; simpl in H8.
+simpl in H6; unfold active in H6; simpl in H6.
+if_tac in H8; auto.
+inversion H8; subst.
+exfalso; apply H6; auto.
+congruence.
+
+(*7*) intros until args; intros H1.
+exists csem; exists (snd w); split; auto.
+
+(*8*) intros until x.
+intros [H1 H2] H3 H4 H5 H6.
+generalize (Extension.csem_wsem_linkable null_extension); intros [_ H10].
+specialize (H10 ef x x).
+specialize (H10 (ext_spec_pre (null_extsig M extension_state 
+  (ext_spec_type signature)) ef x)).
+specialize (H10 (ext_spec_post (null_extsig M extension_state
+  (ext_spec_type signature)) ef x)).
+specialize (H10 P Q).
+spec H10; auto.
+spec H10; auto.
+destruct H10 as [H10 H11].
+specialize (H10 args w m H4); elimtype False; auto.
+
+(*9*) intros until x; intros [H1 H2] H3 H4 H5 H6 H7 [H8 H9]; 
+ intros until j; intros H10; split.
+intros [H11 H12].
+simpl in H12; unfold proj_core in H12; simpl in H12.
+if_tac in H12; auto.
+simpl in H9; unfold proj_core in H9; simpl in H9.
+simpl in H10; unfold active in H10; simpl in H10.
+exfalso; apply H10; auto.
+congruence.
+intros ge n [H11 H12].
+simpl in H10, H12.
+unfold active in H10; unfold proj_core in H12.
+if_tac in H12.
+rewrite H in H10; exfalso; auto.
+congruence.
+Qed.
+
+End NullExtensionSafe.
+
+End NullExtension.
